concurrency/x86_safety.v
@@ -5,10 +5,9 @@ Require Import sepcomp.semantics_lemmas.
 
 Require Import concurrency.pos.
 
-(*
+
 From mathcomp.ssreflect Require Import ssreflect ssrbool ssrnat ssrfun eqtype seq fintype finfun.
 Set Implicit Arguments.
-*)
 
 (*NOTE: because of redefinition of [val], these imports must appear 
   after Ssreflect eqtype.*)
@@ -45,12 +44,12 @@ Module X86Safe.
 
 Section CSPEC.
   Context {cspec: CoreLanguage.corestepSpec}.
-
+  
   Definition csafe (tp : thread_pool) m sched :=
-    forall n, safeN coarse_semantics the_ge n (sched,tp) m.
+    forall n, safety_det coarse_semantics the_ge n (sched,tp) m.
 
   Definition fsafe (tp : thread_pool) m sched :=
-    forall n, safeN fine_semantics the_ge n (sched,tp) m.
+    forall n, safety_det fine_semantics the_ge n (sched,tp) m.
 
   Import Asm Asm_coop.
 
@@ -107,7 +106,7 @@ Proof.
  pose proof (Mem.nextblock_alloc _ _ _ _ _ H).
  apply Mem.alloc_result in H. subst.
  unfold Mem.valid_block in *.
- rewrite H2 in *; clear H2.
+ rewrite H2 in H1; clear H2.
  apply Plt_succ_inv in H1. destruct H1; auto.
  contradiction. subst b'. clear - H.
  Transparent Mem.alloc. unfold Mem.alloc in H. Opaque Mem.alloc.
@@ -126,7 +125,7 @@ Proof.
  right. intro.
  Transparent Mem.alloc. unfold Mem.alloc in H. Opaque Mem.alloc.
   inv H. simpl.
-  rewrite PMap.gso by auto. auto.
+  erewrite PMap.gso by auto. auto.
 *
  revert m H; induction l; intros. inv H. apply decay_refl.
  simpl in H. destruct a. destruct p. 
@@ -156,7 +155,7 @@ Proof.
  assert (~ (lo <= ofs < hi)) by (contradict n; split; auto; omega).
  destruct (zle lo ofs); try reflexivity.
  destruct (zlt ofs hi); try reflexivity. omega.
- rewrite PMap.gso by auto. auto.
+ erewrite PMap.gso by auto. auto.
 *
  apply decay_trans with m''; auto.
  apply mem_step_nextblock in H.
@@ -296,7 +295,7 @@ Opaque Mem.storebytes.
    unfold Mem.valid_block in *.
    eapply Plt_le_trans; eauto.
  }
- rewrite IHmem_step1 by auto. apply IHmem_step2; auto.
+ erewrite IHmem_step1 by auto. apply IHmem_step2; auto.
  contradict H0.
  clear - H H1_ H0.
  revert H H0; induction H1_; intros.
@@ -336,10 +335,355 @@ Instance x86Spec : CoreLanguage.corestepSpec.
 
 End CSPEC.
 
-Parameter init_tp : thread_pool.
-Parameter init_mem : mem.
+Import MemoryWD SimDefs ThreadPoolInjections StepLemmas.
+Definition tpc_init f arg := initial_core coarse_semantics the_ge f arg.
+Definition tpf_init f arg := initial_core fine_semantics the_ge f arg.
+
+(** For now, we assume that the initial memory has no invalid
+pointers, but it should be provable*)
+Axiom init_mem_wd:
+  forall m, init_mem = Some m -> valid_mem m.
+
+(** Also assuming that the initial core will be well-defined*)
+Axiom init_core_wd:
+  forall v args m,
+    init_mem = Some m ->
+    match initial_core SEM.Sem the_ge v args with
+    | Some c => core_wd (id_ren m) c
+    | None => True
+    end.
+
+Lemma init_tp_wd:
+  forall v args m tp,
+    init_mem = Some m ->
+    init_mach init_perm the_ge v args = Some tp ->
+    tp_wd (id_ren m) tp.
+Proof.
+  intros.
+  intros i cnti.
+  unfold init_mach in H0.
+  destruct (initial_core SEM.Sem the_ge v args) eqn:?, init_perm; try discriminate.
+  inversion H0; subst.
+  simpl. split; auto.
+  pose proof (init_core_wd v args H).
+  rewrite Heqo in H1; auto.
+Qed.
+    
+(** Assuming safety of cooperative concurrency*)
+Axiom init_coarse_safe:
+  forall f arg U tpc m,
+    init_mem = Some m ->
+    tpc_init f arg = Some (U, tpc) ->
+  forall (sched : Sch) (n : nat),
+    safeN coarse_semantics the_ge n (sched, tpc) m.
+
+(** If the initial state is defined then the initial memory was also
+defined*)
+Lemma tpc_init_mem_defined:
+  forall f arg U tpc,
+    tpc_init f arg = Some (U, tpc) ->
+    exists m, init_mem = Some m.
+Proof.
+  unfold tpc_init. simpl.
+  unfold myCoarseSemantics.init_machine.
+  unfold init_mach. intros.
+  destruct init_perm eqn:?.
+  unfold init_perm in *.
+  destruct init_mem; try discriminate.
+  eexists; reflexivity.
+  destruct (initial_core SEM.Sem the_ge f arg); try discriminate.
+Qed.
+
+(** The global env is well-defined *)
+Lemma the_ge_wd:
+  forall m,
+    init_mem = Some m ->
+    ge_wd (id_ren m) the_ge.
+Proof.
+  intros. unfold init_mem in H.
+  unfold the_ge.
+  constructor.
+  - intros b Hfuns.
+    destruct ((Genv.genv_funs (Genv.globalenv the_program)) ! b) eqn:Hget;
+      try by exfalso.
+    apply Genv.genv_funs_range in Hget.
+    erewrite Genv.init_mem_genv_next in Hget by eauto.
+    apply id_ren_validblock in Hget.
+    rewrite Hget; auto.
+  - split; intros.
+    destruct ((Genv.genv_vars (Genv.globalenv the_program)) ! b) eqn:Hget;
+      try by exfalso.
+    apply Genv.genv_vars_range in Hget.
+    erewrite Genv.init_mem_genv_next in Hget by eauto.
+    apply id_ren_validblock in Hget.
+    rewrite Hget; auto.
+    unfold Senv.symbol_address in H0.
+    destruct (Senv.find_symbol (Genv.globalenv the_program) id) eqn:Hfind.
+    apply Senv.find_symbol_below in Hfind.
+    unfold Senv.nextblock in Hfind. simpl in Hfind.
+    erewrite Genv.init_mem_genv_next in Hfind by eauto.
+    unfold valid_val. rewrite <- H0.
+    apply id_ren_validblock in Hfind. eexists; eauto.
+    subst. simpl; auto.
+Qed.
+
+(** Simulation relation with id renaming for initial memory*)
+Lemma init_mem_obs_eq :
+  forall m tp f args i (cnti : containsThread tp i)
+    (Hcomp: mem_compatible tp m)
+    (HcompF: mem_compatible tp (diluteMem m)),
+    init_mem = Some m ->
+    init_mach init_perm the_ge f args = Some tp ->
+    mem_obs_eq (id_ren m) (restrPermMap (Hcomp _ cnti))
+               (restrPermMap (HcompF _ cnti)).
+Proof.
+  intros.
+  pose proof (mem_obs_eq_id (init_mem_wd H)) as Hobs_eq_id.
+  unfold init_mach in H0.
+  destruct (initial_core SEM.Sem the_ge f args), init_perm eqn:Hinit_perm;
+    try discriminate.
+  inversion H0; subst.
+  unfold init_perm in Hinit_perm.
+  rewrite H in Hinit_perm.
+  inversion Hinit_perm. subst.
+  destruct Hobs_eq_id.
+  constructor.
+  - constructor;
+    destruct weak_obs_eq0; eauto.
+    intros.
+    do 2 rewrite restrPermMap_Cur.
+    simpl.
+    apply id_ren_correct in Hrenaming. subst.
+    apply po_refl.
+  - constructor.
+    intros.
+    apply id_ren_correct in Hrenaming.
+    subst.
+    do 2 rewrite restrPermMap_Cur.
+    reflexivity.
+    intros.
+    apply id_ren_correct in Hrenaming. subst.
+    eapply memval_obs_eq_id.
+    apply Mem.perm_valid_block in Hperm.
+    simpl.
+    pose proof (init_mem_wd H Hperm ofs ltac:(reflexivity)).
+    destruct (ZMap.get ofs (Mem.mem_contents m) # b2); simpl; auto.
+    rewrite <- wd_val_valid; eauto.
+    apply id_ren_domain.
+    apply id_ren_correct.
+Qed.
+    
+Lemma init_compatible:
+  forall tp f arg m,
+    init_mem = Some m ->
+    init_mach init_perm the_ge f arg = Some tp ->
+    mem_compatible tp m.
+Proof.
+  intros.
+  unfold init_mach in *.
+  destruct (initial_core SEM.Sem the_ge f arg); try discriminate.
+  unfold init_perm in *. rewrite H in H0.
+  inversion H0; subst.
+  constructor.
+  intros j cntj.
+  simpl.
+  unfold permMapLt; intros.
+  apply po_refl.
+  unfold initial_machine. simpl. intros.
+  unfold lockRes in H1.
+  simpl in H1.
+  rewrite threadPool.find_empty in H1. discriminate.
+  unfold initial_machine, lockSet.
+  simpl. unfold addressFiniteMap.A2PMap.
+  simpl.
+  intros b ofs. rewrite Maps.PMap.gi.
+  destruct ((getMaxPerm m) # b ofs); simpl; auto.
+Qed.
+
+Lemma init_thread:
+  forall f arg tp i,
+    init_mach init_perm the_ge f arg = Some tp ->
+    containsThread tp i ->
+    containsThread tp 0.
+Proof.
+  intros.
+  unfold init_mach in *.
+  unfold initial_machine in *.
+  repeat match goal with
+         | [H: match ?Expr with _ => _ end = _ |- _] =>
+           destruct Expr eqn:?; try discriminate
+         end.
+  simpl in H. inversion H; subst.
+  unfold containsThread. simpl.
+  ssromega.
+Qed.
+
+Lemma strong_tsim_refl:
+  forall tp f args m i (cnti: containsThread tp i)
+    (Hcomp: mem_compatible tp m)
+    (HcompF: mem_compatible tp (diluteMem m)),
+    init_mem = Some m ->
+    init_mach init_perm the_ge f args = Some tp ->
+    strong_tsim (id_ren m) cnti cnti Hcomp HcompF.
+Proof.
+  intros.
+  constructor.
+  eapply ctl_inj_id; eauto.
+  pose proof (init_tp_wd f args).
+  specialize (H1 _ _ H H0 i cnti).
+  auto.
+  apply id_ren_correct.
+  eapply init_mem_obs_eq; eauto.
+Qed.
+
+Lemma setMaxPerm_inv:
+  forall m, max_inv (diluteMem m).
+Proof.
+  intros.
+  unfold diluteMem, max_inv, Mem.valid_block, permission_at.
+  intros b ofs H.
+  simpl in H.
+  apply setMaxPerm_MaxV with (ofs := ofs) in H.
+  unfold permission_at in H.
+  auto.
+Qed.
+
+(** Establishing the simulation relation for the initial state*)
+Lemma init_sim:
+  forall f arg U U' tpc tpf m,
+    tpc_init f arg = Some (U, tpc) ->
+    tpf_init f arg = Some (U', tpf) ->
+    init_mem = Some m ->
+    sim tpc m tpf (diluteMem m) nil (id_ren m) (id_ren m) (fun i cnti => id_ren m).
+Proof.
+  intros.
+  unfold tpc_init, tpf_init in *. simpl in *.
+  unfold myCoarseSemantics.init_machine, myFineSemantics.init_machine in *.
+  destruct (init_mach init_perm the_ge f arg) eqn:Hinit; try discriminate.
+  inversion H; subst. inversion H0; subst.
+  clear H H0.
+  assert (HmemComp := init_compatible f arg H1 Hinit).
+  assert (HmemCompF: mem_compatible tpf (diluteMem m))
+    by (eapply mem_compatible_setMaxPerm; eauto).
 
 
+  eapply Build_sim with (mem_compc := HmemComp) (mem_compf := HmemCompF).
+  - intros; split; auto.
+  - eapply init_coarse_safe with (f := f) (arg := arg); eauto.
+    unfold tpc_init. simpl. unfold myCoarseSemantics.init_machine.
+    rewrite Hinit. reflexivity. 
+  - intros i cnti cnti'.
+    pose proof (strong_tsim_refl _ _ cnti HmemComp HmemCompF H1 Hinit).
+    pf_cleanup.
+    destruct H. destruct obs_eq0.
+    eauto.
+  - intros; by congruence.
+  - intros.
+    exists tpf, m.
+    split; eauto with renamings.
+    split; eauto.
+    split; first by constructor.
+    split.
+    intros; pf_cleanup.
+    eapply strong_tsim_refl; eauto.
+    repeat (split; intros); congruence.
+  - unfold init_mach in *.
+    unfold init_perm in Hinit.
+    rewrite H1 in Hinit.
+    destruct (initial_core SEM.Sem the_ge f arg); try discriminate.
+    inversion Hinit; subst.
+    split.
+    constructor.
+    intros.
+    do 2 rewrite restrPermMap_Cur.
+    unfold initial_machine, lockSet. simpl.
+    unfold addressFiniteMap.A2PMap. simpl.
+    do 2 rewrite Maps.PMap.gi; reflexivity.
+    intros.
+    assert (Heq := restrPermMap_Cur (compat_ls HmemComp) b1 ofs).
+    unfold permission_at in Heq.
+    unfold Mem.perm in Hperm.
+    rewrite Heq in Hperm.
+    unfold lockSet, initial_machine, addressFiniteMap.A2PMap in Hperm.
+    simpl in Hperm.
+    rewrite Maps.PMap.gi in Hperm.
+    simpl in Hperm. exfalso; auto.
+    intros. unfold lockRes, initial_machine in H. simpl in H.
+      by exfalso.
+  - intros.
+    unfold init_mach, init_perm in Hinit.
+    rewrite H1 in Hinit.
+    destruct (initial_core SEM.Sem the_ge f arg); try discriminate.
+    inversion Hinit; subst.
+    unfold lockRes, initial_machine in Hl1.
+    simpl in Hl1;
+      by exfalso.
+  - unfold init_mach, init_perm in Hinit.
+    rewrite H1 in Hinit.
+    destruct (initial_core SEM.Sem the_ge f arg); try discriminate.
+    inversion Hinit; subst.
+    apply DryMachineLemmas.initial_invariant.
+  - apply setMaxPerm_inv; auto.
+  - apply init_mem_wd; auto.
+  - eapply init_tp_wd; eauto.
+  - unfold the_ge.
+    eapply the_ge_wd; eauto.
+  - split; eauto with renamings.
+    apply id_ren_correct.
+  - simpl. tauto.
+Qed.
+
+(** Safety of the FineConc machine*)
+
+Import StepType.
+
+Lemma fine_safe:
+  forall tpf tpc mf mc (f fg : memren) fp (xs : Sch)
+    (Hsim: sim tpc mc tpf mf xs f fg fp),
+  forall sched n,
+    safeN fine_semantics the_ge n (sched, tpf) mf.
+Proof.
+  intros.
+  generalize dependent xs.
+  induction n; intros; simpl; auto.
+  destruct sched as [|i sched]; simpl; auto.
+  Definition containsThread_dec:
+    forall i tp, {containsThread tp i} + { ~ containsThread tp i}.
+  Proof.
+    intros.
+    unfold containsThread.
+    destruct (leq (S i) (num_threads tp)) eqn:Hleq;
+      by auto.
+  Qed.
+  destruct (containsThread_dec i tpf) as [cnti | invalid].
+  - (* By case analysis on the step type *)
+    destruct (getStepType cnti) eqn:Htype.
+    + pose proof (sim_internal cnti Htype Hsim) as (tpf' & m' & fp' & Hstep & Hsim').
+      split.
+      exists (sched,tpf'), m'.
+      eapply Hstep.
+      intros (U' & tpf'') mf'' Hstep'.
+      
+      
+      
+
+Theorem init_fine_safe:
+  forall f arg U tpf m
+    (Hmem: init_mem = Some m)
+    (Hinit: tpf_init f arg = Some (U, tpf)),
+    forall (sched : Sch) (n : nat),
+      safeN fine_semantics the_ge n (sched, tpf) m.
+Proof.
+  intros.
+  assert (Hsim := init_sim f arg Hinit Hinit Hmem).
+  clear - Hsim.
+  generalize dependent m. generalize dependent tpf.
+  induction n; simpl; auto.
+  intros.
+  destruct sched
+  
+      
+                       
 
 End X86Safe.
 
